---
layout: post
title:  "Time Series Analysis"
date:  2016-04-22 21:00:00
tag:
- Statistics
- Note
blog: true
author: Jannis
description: simple AR(1) model
fontsize: 23pt
---

{% include mathjax_support_1.html %}

For AR(1) process,
$$X_{t} = - \sum_{j=1}^{\infty}\phi^{-j}Z_{t+j}$$
where $$\{Z_{t}\} \sim WN(0,\sigma^{2})$$, $$\mid{\phi}\mid > 1$$.

First we can derive the $$\gamma_{X}(0)$$  since $${Z_{t}}$$ are uncorrelated to each other.

<div>
$$
\begin{align}
\gamma_{x}(0)
& = Var(X_{t}) = Var( - \sum_{j=1}^{\infty}\phi^{-j}Z_{t+j}) = Var( \sum_{j=1}^{\infty}\phi^{-j}Z_{t+j}) \\\\
& = \sum_{j=1}^{\infty}Var(\phi^{-j}Z_{t+j}) = \sum_{j=1}^{\infty}(\phi^{-j})^{2}Var(Z_{t+j}) = \sum_{j=1}^{\infty}(\phi^{-j})^{2}\sigma^{2} \\\\
& = \sum_{j=1}^{\infty}\phi^{-2j}\sigma^{2} = \sigma^{2}\sum_{j=1}^{\infty}\phi^{-2j} = \sigma^{2}\frac{\phi^{-2}}{1-\phi^{-2}} =\frac{\sigma^{2}}{\phi^{2} - 1}
\end{align}
$$
</div>

Then AR(1) model can also be written as

$$X_{t} = Z_{t} + \phi X_{t-1}$$

But since $$\mid\phi\mid > 1$$, so we interpret it in another way

$$X_{t+1}= Z_{t+1} + \phi X_{t}$$

$$\phi^{-1}X_{t+1} = \phi^{-1}Z_{t+1} +  X_{t}$$

$$X_{t} = \phi^{-1}X_{t+1} - \phi^{-1}Z_{t+1}$$

So we plug it in $\gamma_{x}(h)$, $(h > 0)$

<div> $$
\begin{align}
\gamma_{x}(h)
& = \gamma_{x}(X_{t+h},X_{t}) \\\\
& =Cov(X_{t+h},\phi^{-1}X_{t+1} - \phi^{-1}Z_{t+1}) \\\\
& = Cov(X_{t+h},\phi^{-1}X_{t+1}) - Cov(X_{t+h},\phi^{-1}Z_{t+1}) \\\\
& = \phi^{-1}Cov(X_{t+h},X_{t+1}) - \phi^{-1}Cov(X_{t+h},Z_{t+1}) \\\\
& = \phi^{-1}\gamma_{x}(h-1) - \phi^{-1}Cov(X_{t+h},Z_{t+1})
\end{align}
$$ </div>

We also know that $Cov(X_{s},Z_{t}) = 0$ if $s \geq t$ since

$$X_{t} = - \sum_{j=1}^{\infty}\phi^{-j}Z_{t+j}$$

$$Cov(X_{s},Z_{t}) = Cov(- \sum_{j=1}^{\infty}\phi^{-j}Z_{s+j},Z_{t}) $$

where $s \geq t$. So $s + j > t$ for j = 1, 2, ...

Hence $Cov(X_{s},Z_{t}) = 0$ if $s \geq t$

Therefore,

$$\gamma_{x}(h) = \phi^{-1}\gamma_{x}(h-1)$$

By induction, we know that

$$\gamma_{x}(h) = \phi^{-h}\gamma_{X}(0)$$

Then plug $$\gamma_{x}(0)$$ in equation we can get

$$\gamma_{x}(h) = \phi^{-h}\frac{\sigma^{2}}{\phi^{2} - 1}
 = \frac{\sigma^{2}}{\phi^{h}(\phi^{2} - 1)}$$
